refactor mem to use nat-based address

src/Mem.v
@@ -1,55 +1,159 @@
+Require Import Arith.
+Require Import Word.
+Require Import Bytes.
+Require Import Eqdep_dec.
 Require Import FunctionalExtensionality.
 
 Set Implicit Arguments.
 
+Definition EqDec (T : Type) := forall (a b : T), {a = b} + {a <> b}.
 
-Definition DecEq (T : Type) := forall (a b : T), {a=b}+{a<>b}.
-Definition mem {A : Type} {eq : DecEq A} {V: Type} := A -> option V.
-Definition upd {A : Type} {eq : DecEq A} {V: Type} (m : @mem A eq V) (a : A) (v : V) : @mem A eq V :=
-  fun a' => if eq a' a then Some v else m a'.
-Definition upd_none {A : Type} {eq : DecEq A} {V : Type} (m : @mem A eq V) (a : A) : @mem A eq V :=
-  fun a' => if eq a' a then None else m a'.
+(* generalized memory of any address / value type *)
 
-Definition empty_mem {AT : Type} {AEQ : DecEq AT} {V : Type} : @mem AT AEQ V := fun a => None.
+Section GENMEM.
+  Variable A : Type.
+  Variable V : Type.
+  Variable AEQ : EqDec A.
+
+  Definition mem := A -> option V.
+  Definition upd (m : mem) (a : A) (v : V) : mem :=
+    fun a' => if AEQ a' a then Some v else m a'.
+
+  Definition upd_none (m : mem) (a : A) : mem :=
+    fun a' => if AEQ a' a then None else m a'.
+
+  Definition empty_mem : mem := fun a => None.
+
+  Theorem upd_eq : forall m (a : A) (v : V) a',
+    a' = a -> upd m a v a' = Some v.
+  Proof.
+    intros; subst; unfold upd.
+    destruct (AEQ a a); tauto.
+  Qed.
+
+  Theorem upd_ne : forall m (a : A) (v:V) a',
+    a' <> a
+    -> upd m a v a' = m a'.
+  Proof.
+    intros; subst; unfold upd.
+    destruct (AEQ a' a); tauto.
+  Qed.
+
+  Theorem upd_repeat: forall m (a : A) (v v':V),
+    upd (upd m a v') a v = upd m a v.
+  Proof.
+    intros; apply functional_extensionality; intros.
+    case_eq (AEQ a x); intros; subst.
+    repeat rewrite upd_eq; auto.
+    repeat rewrite upd_ne; auto.
+  Qed.
+
+  Theorem upd_comm: forall m (a0 : A) (v0 : V) a1 v1, a0 <> a1
+    -> upd (upd m a0 v0) a1 v1 = upd (upd m a1 v1) a0 v0.
+  Proof.
+    intros; apply functional_extensionality; intros.
+    case_eq (AEQ a1 x); case_eq (AEQ a0 x); intros; subst; try congruence;
+    repeat ( ( rewrite upd_ne by auto ) || ( rewrite upd_eq by auto ) ); auto.
+  Qed.
+
+End GENMEM.
 
 
-Section GenMem.
 
-Variable V : Type.
-Variable A : Type.
-Variable aeq : DecEq A.
+(* Disk value and address types  *)
 
-Theorem upd_eq : forall m (a : A) (v:V) a',
-  a' = a
-  -> @upd A aeq V m a v a' = Some v.
+Notation "'valubytes_real'" := 4096. (* 4KB *)
+Notation "'valulen_real'" := (valubytes_real * 8)%nat.
+
+Module Type VALULEN.
+  Parameter valulen : nat.
+  Parameter valubytes : nat.
+  Axiom valulen_is : valulen = valulen_real.
+  Axiom valubytes_is : valubytes = valubytes_real.
+End VALULEN.
+
+Module Valulen : VALULEN.
+  Definition valulen := valulen_real.
+  Definition valubytes := valubytes_real.
+  Theorem valulen_is: valulen = valulen_real.
+  Proof.
+    auto.
+  Qed.
+  Theorem valubytes_is: valubytes = valubytes_real.
+  Proof.
+    auto.
+  Qed.
+End Valulen.
+
+Definition addrlen := 64.
+Notation "'valulen'" := (Valulen.valulen).
+Notation "'valubytes'" := (Valulen.valubytes).
+Notation "'valulen_is'" := (Valulen.valulen_is).
+Notation "'valubytes_is'" := (Valulen.valubytes_is).
+
+Notation "'addr'" := nat.
+Notation "'waddr'" := (word addrlen).
+Notation "'valu'" := (word valulen).
+
+Definition addr_eq_dec := Nat.eq_dec.
+Definition waddr_eq_dec := @weq addrlen.
+
+Definition valu2bytes (v : valu) : bytes valubytes.
+  refine (@word2bytes valulen valubytes _ v).
+  rewrite valulen_is. rewrite valubytes_is. reflexivity.
+Defined.
+
+Definition bytes2valu (v : bytes valubytes) : valu.
+  rewrite valulen_is.
+  unfold bytes in *.
+  rewrite valubytes_is in *.
+  exact v.
+Defined.
+
+Theorem valu2bytes2valu : forall v, valu2bytes (bytes2valu v) = v.
 Proof.
-  intros; subst; unfold upd.
-  destruct (aeq a a); tauto.
+  unfold valu2bytes, bytes2valu, eq_rec_r, eq_rec.
+  intros.
+  rewrite eq_rect_word_mult.
+  rewrite eq_rect_nat_double.
+  generalize dependent v.
+  rewrite valubytes_is.
+  rewrite valulen_is.
+  intros.
+  rewrite <- (eq_rect_eq_dec eq_nat_dec).
+  reflexivity.
 Qed.
 
-Theorem upd_ne : forall m (a : A) (v:V) a',
-  a' <> a
-  -> @upd A aeq V m a v a' = m a'.
+Theorem bytes2valu2bytes : forall v, bytes2valu (valu2bytes v) = v.
 Proof.
-  intros; subst; unfold upd.
-  destruct (aeq a' a); tauto.
+  unfold valu2bytes, bytes2valu, eq_rec_r, eq_rec.
+  intros.
+  rewrite eq_rect_word_mult.
+  rewrite eq_rect_nat_double.
+  generalize dependent v.
+  rewrite valubytes_is.
+  rewrite valulen_is.
+  intros.
+  rewrite <- (eq_rect_eq_dec eq_nat_dec).
+  reflexivity.
 Qed.
 
-Theorem upd_repeat: forall m (a : A) (v v':V),
-  upd (@upd A aeq V m a v') a v = upd m a v.
+Theorem valulen_wordToNat_natToWord : # (natToWord addrlen valulen) = valulen.
 Proof.
-  intros; apply functional_extensionality; intros.
-  case_eq (aeq a x); intros; subst.
-  repeat rewrite upd_eq; auto.
-  repeat rewrite upd_ne; auto.
+  rewrite valulen_is.
+  compute.
+  reflexivity.
 Qed.
 
-Theorem upd_comm: forall m (a0 : A) (v0:V) a1 v1, a0 <> a1
-  -> upd (@upd A aeq V m a0 v0) a1 v1 = upd (upd m a1 v1) a0 v0.
+(* tight bound for valulen *)
+Theorem valulen_bound : valulen < pow2 16.
 Proof.
-  intros; apply functional_extensionality; intros.
-  case_eq (aeq a1 x); case_eq (aeq a0 x); intros; subst; try congruence;
-  repeat ( ( rewrite upd_ne by auto ) || ( rewrite upd_eq by auto ) ); auto.
+  eapply Nat.lt_le_trans with (m := pow2 15 + 1).
+  rewrite valulen_is.
+  compute; auto.
+  apply pow2_le_S.
 Qed.
 
-End GenMem.
+
+Definition wringaddr := wring addrlen.
+Add Ring wringaddr : wringaddr (decidable (weqb_sound addrlen), constants [wcst]).
